JVM m5: Linking preprocessor creates array classes referenced in classfiles

books/models/jvm/m5/Apprentice.java
@@ -24,7 +24,7 @@ class Job extends Thread {
 }
 
 class Apprentice {
-    public static void main(String[] args) {
+    public static void main(/*String[] args*/) {
 
         Container container = new Container();
 
