books/models/jvm/m5/jvm-fact-setup.lisp
@@ -154,28 +154,35 @@ The output of jvm2acl2 for M5 is in classes/Demo.
  ((0 ("java/lang/Class" ("<name>" . "java/lang/Object"))
      ("java/lang/Object" ("<monitor>" . 0)
                          ("<mcount>" . 0)))
-  (1 ("java/lang/Class" ("<name>" . "ARRAY"))
+  (1 ("java/lang/Class" ("<name>" . "[Ljava/lang/Object;"))
      ("java/lang/Object" ("<monitor>" . 0)
                          ("<mcount>" . 0)))
-  (2 ("java/lang/Class" ("<name>" . "java/lang/Thread"))
+  (2 ("java/lang/Class" ("<name>" . "[C"))
      ("java/lang/Object" ("<monitor>" . 0)
                          ("<mcount>" . 0)))
-  (3 ("java/lang/Class" ("<name>" . "java/lang/String"))
+  (3 ("java/lang/Class" ("<name>" . "java/lang/Thread"))
      ("java/lang/Object" ("<monitor>" . 0)
                          ("<mcount>" . 0)))
-  (4 ("java/lang/Class" ("<name>" . "java/lang/Class"))
+  (4 ("java/lang/Class" ("<name>" . "java/lang/String"))
      ("java/lang/Object" ("<monitor>" . 0)
                          ("<mcount>" . 0)))
-  (5 ("java/lang/Class" ("<name>" . "Demo")
+  (5 ("java/lang/Class" ("<name>" . "[Ljava/lang/String;"))
+     ("java/lang/Object" ("<monitor>" . 0)
+                         ("<mcount>" . 0)))
+  (6 ("java/lang/Class" ("<name>" . "java/lang/Class"))
+     ("java/lang/Object" ("<monitor>" . 0)
+                         ("<mcount>" . 0)))
+  (7 ("java/lang/Class" ("<name>" . "Demo")
                         ("ans:I" . 0))
      ("java/lang/Object" ("<monitor>" . 0)
                          ("<mcount>" . 0))))
  (("java/lang/Object" NIL NIL
                       NIL NIL (("<init>:()V" NIL (RETURN)))
                       (REF 0))
-  ("ARRAY" ("java/lang/Object")
-           (("<array>" . *ARRAY*))
-           NIL NIL NIL (REF 1))
+  ("[Ljava/lang/Object;" ("java/lang/Object")
+                         NIL NIL NIL NIL (REF 1))
+  ("[C" ("java/lang/Object")
+        NIL NIL NIL NIL (REF 2))
   ("java/lang/Thread"
        ("java/lang/Object")
        NIL NIL NIL
@@ -185,7 +192,7 @@ The output of jvm2acl2 for M5 is in classes/Demo.
         ("<init>:()V" NIL (ALOAD_0)
                       (INVOKESPECIAL "java/lang/Object" "<init>:()V" 0)
                       (RETURN)))
-       (REF 2))
+       (REF 3))
   ("java/lang/String"
        ("java/lang/Object")
        ("value:[C")
@@ -193,14 +200,16 @@ The output of jvm2acl2 for M5 is in classes/Demo.
        (("<init>:()V" NIL (ALOAD_0)
                       (INVOKESPECIAL "java/lang/Object" "<init>:()V" 0)
                       (RETURN)))
-       (REF 3))
+       (REF 4))
+  ("[Ljava/lang/String;" ("[Ljava/lang/Object;" "java/lang/Object")
+                         NIL NIL NIL NIL (REF 5))
   ("java/lang/Class"
        ("java/lang/Object")
        NIL NIL NIL
        (("<init>:()V" NIL (ALOAD_0)
                       (INVOKESPECIAL "java/lang/Object" "<init>:()V" 0)
                       (RETURN)))
-       (REF 4))
+       (REF 6))
   ("Demo" ("java/lang/Object")
           NIL ("ans:I")
           NIL
@@ -241,7 +250,7 @@ The output of jvm2acl2 for M5 is in classes/Demo.
                 (INVOKEVIRTUAL "NoClassDefFoundError: java/io/PrintStream"
                                "println:(I)V" 1)
                 (RETURN)))
-          (REF 5)))
+          (REF 7)))
  DEFAULT-M5-OPTIONS)
 |#
 
@@ -276,33 +285,44 @@ The output of jvm2acl2 for M5 is in classes/Demo.
 (defconst *Demo-heap*
   '((0 . (("java/lang/Class" ("<name>" . "java/lang/Object"))
           ("java/lang/Object" ("<monitor>" . 0) ("<mcount>" . 0))))
-    (1 . (("java/lang/Class" ("<name>" . "ARRAY"))
+    (1 . (("java/lang/Class" ("<name>" . "[Ljava/lang/Object;"))
           ("java/lang/Object" ("<monitor>" . 0) ("<mcount>" . 0))))
-    (2 . (("java/lang/Class" ("<name>" . "java/lang/Thread"))
+    (2 . (("java/lang/Class" ("<name>" . "[C"))
           ("java/lang/Object" ("<monitor>" . 0) ("<mcount>" . 0))))
-    (3 . (("java/lang/Class" ("<name>" . "java/lang/String"))
+    (3 . (("java/lang/Class" ("<name>" . "java/lang/Thread"))
           ("java/lang/Object" ("<monitor>" . 0) ("<mcount>" . 0))))
-    (4 . (("java/lang/Class" ("<name>" . "java/lang/Class"))
+    (4 . (("java/lang/Class" ("<name>" . "java/lang/String"))
           ("java/lang/Object" ("<monitor>" . 0) ("<mcount>" . 0))))
-    (5 . (("java/lang/Class" ("<name>" . "Demo") ("ans:I" . 0))
+    (5 . (("java/lang/Class" ("<name>" . "[Ljava/lang/String;"))
+          ("java/lang/Object" ("<monitor>" . 0) ("<mcount>" . 0))))
+    (6 . (("java/lang/Class" ("<name>" . "java/lang/Class"))
+          ("java/lang/Object" ("<monitor>" . 0) ("<mcount>" . 0))))
+    (7 . (("java/lang/Class" ("<name>" . "Demo") ("ans:I" . 0))
           ("java/lang/Object" ("<monitor>" . 0) ("<mcount>" . 0))))))
 
 (defconst *Demo-class-table*
   '(("java/lang/Object"
      NIL
-     ()
+     NIL
      NIL
      NIL
      (("<init>:()V" NIL
        (RETURN)))
      (REF 0))
-    ("ARRAY"
+    ("[Ljava/lang/Object;"
      ("java/lang/Object")
-     (("<array>" . *ARRAY*))
+     NIL
      NIL
      NIL
      NIL
      (REF 1))
+    ("[C"
+     ("java/lang/Object")
+     NIL
+     NIL
+     NIL
+     NIL
+     (REF 2))
     ("java/lang/Thread"
      ("java/lang/Object")
      NIL
@@ -318,7 +338,7 @@ The output of jvm2acl2 for M5 is in classes/Demo.
        (ALOAD\_0)
        (INVOKESPECIAL "java/lang/Object" "<init>:()V" 0)
        (RETURN)))
-     (REF 2))
+     (REF 3))
     ("java/lang/String"
      ("java/lang/Object")
      ("value:[C")
@@ -328,7 +348,14 @@ The output of jvm2acl2 for M5 is in classes/Demo.
        (ALOAD\_0)
        (INVOKESPECIAL "java/lang/Object" "<init>:()V" 0)
        (RETURN)))
-     (REF 3))
+     (REF 4))
+    ("[Ljava/lang/String;"
+     ("[Ljava/lang/Object;" "java/lang/Object")
+     NIL
+     NIL
+     NIL
+     NIL
+     (REF 5))
     ("java/lang/Class"
      ("java/lang/Object")
      NIL
@@ -338,7 +365,7 @@ The output of jvm2acl2 for M5 is in classes/Demo.
        (ALOAD\_0)
        (INVOKESPECIAL "java/lang/Object" "<init>:()V" 0)
        (RETURN)))
-     (REF 4))
+     (REF 6))
     ("Demo"
      ("java/lang/Object")
      NIL
@@ -381,7 +408,7 @@ The output of jvm2acl2 for M5 is in classes/Demo.
        (INVOKESTATIC "Demo" "fact:(I)I" 1)
        (INVOKEVIRTUAL "NoClassDefFoundError: java/io/PrintStream" "println:(I)V" 1)
        (RETURN)))
-     (REF 5))))
+     (REF 7))))
 
 (defconst *Demo-state*
   (make-state *demo-thread-table*
